theories/c_toy_lang/melocoton/examples.v
@@ -9,7 +9,7 @@ Import uPred.
 (** Heap tactics *)
 Section examples.
 
-Context `{!heapGS_gen hlc Σ}.
+Context `{!heapGS_C_gen hlc Σ}.
  
 Fixpoint fib (n:nat) : nat := match n with
   0 => 0
@@ -41,7 +41,7 @@ Notation FibSpec name := (λ (s:string) (v:list val) (Φ : (val → iPropI Σ)),
     | _ => ⌜False⌝%I end).
 
 Definition StoreItSpec := λ s v Φ, match (s,v) with
-      ("store_it", [ #(LitLoc l) ; v' ]) => (∃ v, (l I↦ v) ∗ ((l ↦{DfracOwn 1} v') -∗ Φ (#0)))%I
+      ("store_it", [ #(LitLoc l) ; v' ]) => (∃ v, (l I↦ v) ∗ ((l ↦C v') -∗ Φ (#0)))%I
     | _ => ⌜False⌝%I end.
 
 Definition FibLeftSpec := FibSpec "fib_left".
